Optimizations/Canonicalizations/AbsPhase.thy
@@ -13,8 +13,8 @@ text \<open>
 Note:
 
 We can't use @{const word_sless} for reasoning about @{const intval_less_than}.
-@{const word_sless} will always treat the 64^{th} bit as the sign flag
-while @{const intval_less_than} uses the b^{th} bit depending on the size of the word.
+@{const word_sless} will always treat the $64^{th}$ bit as the sign flag
+while @{const intval_less_than} uses the $b^{th}$ bit depending on the size of the word.
 \<close>
 
 value "val[new_int 32 0 < new_int 32 4294967286]" \<comment> \<open>0 < -10 = False\<close>
@@ -60,11 +60,6 @@ value "-(set_bit 1 0)::2 word" \<comment> \<open>2\<close>
 value "(set_bit 31 0)::32 word" \<comment> \<open>2147483648\<close>
 value "-(set_bit 31 0)::32 word" \<comment> \<open>2147483648\<close>
 
-lemma negate_horner:
-  fixes v :: "'a::len word"
-  shows "-v = (horner_sum of_bool 2 (map (\<lambda>i. \<not>(bit v i)) [0..<LENGTH('a)])) + 1"
-  sorry
-
 
 lemma negative_def:
   fixes v :: "'a::len word"
@@ -80,23 +75,110 @@ lemma positive_def:
   using assms
   by (simp add: bit_last_iff word_sless_alt)
 
+(*
+lemma invert1:
+  fixes v :: "'a::len word"
+  assumes "v <s 0"
+  assumes "v > (2^(LENGTH('a) - 1))"
+  shows "0 <s (-v)"
+proof -
+  have "-v = Word.Word (-(Word.rep v))"
+    by (metis uminus_word.abs_eq unsigned.abs_eq unsigned.rep_eq word_minus_def)
+  have "v < 0 \<longrightarrow> 0 < (-(Word.rep v))"
+    by auto
+  have negbit: "bit v (LENGTH('a) - 1)"
+    using assms(1) negative_def by blast
+  then have "0 <s (-v) = (0 < signed_take_bit (LENGTH('a) - 1) (Word.rep (-v)))"
+    unfolding word_sless_def apply simp
+    by (metis id_apply of_int_eq_id signed.rep_eq sint_0)
+  have "signed_take_bit (LENGTH('a) - 1) (Word.rep v) = (or (take_bit (LENGTH('a) - 1) (Word.rep v)) (not (mask (LENGTH('a) - 1))))"
+    using signed_take_bit_eq_if_negative negbit
+    by (metis bit_word.rep_eq)
+  then have "0 <s (-v) = (0 < (or (take_bit (LENGTH('a) - 1) (Word.rep (-v))) (not (mask (LENGTH('a) - 1)))))"
+    unfolding word_sless_def apply simp using signed_take_bit_eq_if_negative negbit sorry
+  have "0 < (-(Word.rep v) mod 2^(LENGTH('a) - 1)) \<longrightarrow> 0 <s (-v)"
+    unfolding word_sless_def sorry
+  then show ?thesis sorry
+qed
+
+value "1::1 word"
+value "2^(1 - 1)::1 word"
+value "bit (1::1 word) 1"
+
+lemma
+  fixes v :: "'a::len word"
+  shows "v \<ge> (2^(LENGTH('a) - 1)) \<Longrightarrow> bit v (LENGTH('a) - 1)"
+  sorry
+
+lemma negative_lower_bound:
+  fixes v :: "'a::len word"
+  assumes "v <s 0"
+  shows "v \<ge> (2^(LENGTH('a) - 1))"
+  using assms unfolding word_sless_def
+  apply auto sorry
+
 lemma invert:
   fixes v :: "'a::len word"
   assumes "v <s 0"
-  assumes "v \<noteq> (set_bit (LENGTH('a) - 1) 0)"
+  assumes "v \<noteq> (2^(LENGTH('a) - 1))"
   shows "0 <s (-v)"
-proof -
-  have negBitSet: "bit v (LENGTH('a) - 1)"
-    using assms(1)
-    using negative_def by blast
-  have "v = (horner_sum of_bool 2 (map (\<lambda>i. (bit v i)) [0..<LENGTH('a)]))"
-    by (simp add: horner_sum_bit_eq_take_bit)
-  then have "-v = (horner_sum of_bool 2 (map (\<lambda>i. \<not>(bit v i)) [0..<LENGTH('a)])) + 1"
-    using negate_horner by blast
-  then have "\<not>(bit v (LENGTH('a) - 1))"
-    sorry
+  using invert1 assms negative_lower_bound order_less_le by blast
+*)
+
+lemma negative_lower_bound:
+  fixes v :: "'a::len word"
+  assumes "(2^(LENGTH('a) - 1)) <s v"
+  assumes "v <s 0"
+  shows "0 <s (-v)"
+  using assms
+  by (smt (verit) signed_0 signed_take_bit_int_less_self_iff sint_ge sint_word_ariths(4) word_sless_alt)
+
+lemma min_int:
+  fixes x :: "'a::len word"
+  assumes "x <s 0"
+  assumes "x \<noteq> (2^(LENGTH('a) - 1))"
+  shows "2^(LENGTH('a) - 1) <s x"
+  using assms sorry
+
+(*
+lemma min_int:
+  fixes x :: "'a::len word"
+  assumes "x <s 0 \<and> 0 <s x"
+  shows "x = 2^(LENGTH('a) - 1)"
+  using assms
+  using signed.less_asym by blast
+*)
+
+lemma negate_min_int:
+  fixes v :: "'a::len word"
+  assumes "v = (2^(LENGTH('a) - 1))"
+  shows "v = (-v)"
+  using assms
+  by (metis One_nat_def add.inverse_neutral double_eq_zero_iff mult_minus_right verit_minus_simplify(4))
+
+fun abs :: "'a::len word \<Rightarrow> 'a word" where
+  "abs x = (if x <s 0 then (-x) else x)"
+
+lemma
+  "abs(abs(x)) = abs(x)"
+  for x :: "'a::len word"
+proof (cases "0 \<le>s x")
+  case True
   then show ?thesis
-    using negBitSet by blast
+    by force
+next
+  case neg: False
+  then show ?thesis
+  proof (cases "x = (2^LENGTH('a) - 1)")
+    case True
+    then show ?thesis
+      using negate_min_int
+      by (simp add: word_sless_alt)
+  next
+    case False
+    then show ?thesis using min_int negative_lower_bound
+      using negate_min_int by force
+  qed
 qed
 
 text \<open>We need to do the same proof at the value level.\<close>
@@ -105,21 +187,21 @@ lemma invert_intval:
   assumes "int_signed_value b v < 0"
   assumes "b > 0 \<and> b \<le> 64"
   assumes "take_bit b v = v"
-  assumes "v \<noteq> (set_bit (b - 1) 0)"
+  assumes "v \<noteq> (2^(b - 1))"
   shows "0 < int_signed_value b (-v)"
   using assms apply simp sorry
 
 lemma negate_max_negative:
   assumes "b > 0 \<and> b \<le> 64"
   assumes "take_bit b v = v"
-  assumes "v = (set_bit (b - 1) 0)"
+  assumes "v = (2^(b - 1))"
   shows "new_int b v = intval_negate (new_int b v)"
-  using assms apply simp sorry
+  using assms apply simp using negate_min_int sorry
 
 lemma val_abs_always_pos:
   assumes "b > 0 \<and> b \<le> 64"
   assumes "take_bit b v = v"
-  assumes "v \<noteq> (set_bit (b - 1) 0)"
+  assumes "v \<noteq> (2^(b - 1))"
   assumes "intval_abs (new_int b v) = (new_int b v')"
   shows "val_to_bool (val[(new_int b 0) < (new_int b v')]) \<or> val_to_bool (val[(new_int b 0) eq (new_int b v')])"
 proof (cases "v = 0")
@@ -208,7 +290,7 @@ proof -
   proof (cases "int_signed_value b v < 0")
     case neg: True
     then show ?thesis
-    proof (cases "v = (set_bit (b - 1) 0)")
+    proof (cases "v = (2^(b - 1))")
       case min: True
       then show ?thesis
         by (smt (z3) assms(1) bInRange in_def intval_abs.simps(1) intval_negate.simps(1) negate_max_negative new_int.simps valid_value.simps(1))
@@ -233,10 +315,12 @@ qed
 
 paragraph \<open>Optimisations\<close>
 
+(*
 optimization AbsIdempotence:
   "abs(abs(x)) \<longmapsto> abs(x) when wf_stamp x \<and> stamp_expr x = IntegerStamp b l h"
   using val_abs_idem
   using wf_stamp_def by fastforce
+*)
 
 end
 
