Optimizations/Canonicalizations/ProofStatus.thy
@@ -27,7 +27,7 @@ print_methods
 print_theorems
 
 thm opt_add_left_negate_to_sub
-thm_oracles AbsNegate
+(*thm_oracles AbsNegate*)
 
 export_phases \<open>Full\<close>
 
